expose a bug in ecancel in ARPResponderProofs

bedrock2/src/Examples/ARPResponder.v
@@ -14,53 +14,52 @@ Definition arp : bedrock_func :=
     let buf : varname := "buf" in
     let len : varname := "len" in
   ("arp", ([ethbuf; len], [], bedrock_func_body:(
-    buf = (ethbuf+constr:(14));
     require ( constr:(14+27) < len ) else { /*skip*/ };
-    require ( (load1(buf)            == constr:(0))
-            & (load1(buf+constr:(1)) == constr:(1))
-            & (load1(buf+constr:(2)) == constr:(Ox"08"))
-            & (load1(buf+constr:(3)) == constr:(0))
-            & (load1(buf+constr:(4)) == constr:(6))
-            & (load1(buf+constr:(5)) == constr:(4))
+    require ( (load1(ethbuf+constr:(14+0))== constr:(0))
+            & (load1(ethbuf+constr:(14+1)) == constr:(1))
+            & (load1(ethbuf+constr:(14+2)) == constr:(Ox"08"))
+            & (load1(ethbuf+constr:(14+3)) == constr:(0))
+            & (load1(ethbuf+constr:(14+4)) == constr:(6))
+            & (load1(ethbuf+constr:(14+5)) == constr:(4))
             ) else { /*skip*/ };
     (* TODO: update sender mapping if present *)
-    require ( (load1(buf+constr:(6)) == constr:(0))
-            & (load1(buf+constr:(6+1)) == constr:(1))
+    require ( (load1(ethbuf+constr:(14+6)) == constr:(0))
+            & (load1(ethbuf+constr:(14+6+1)) == constr:(1))
             ) else { /*skip*/ }; (* request *)
-    store1(buf+constr:(6+1), constr:(2)); (* response *)
+    store1(ethbuf+constr:(14+6+1), constr:(2)); (* response *)
     (* TODO: add sender mapping to arp table *)
 
     (* dst := src *)
-    store1(buf+constr:(18  ), load1(buf+constr:(8  )));
-    store1(buf+constr:(18+1), load1(buf+constr:(8+1)));
-    store1(buf+constr:(18+2), load1(buf+constr:(8+2)));
-    store1(buf+constr:(18+3), load1(buf+constr:(8+3)));
-    store1(buf+constr:(18+4), load1(buf+constr:(8+4)));
-    store1(buf+constr:(18+5), load1(buf+constr:(8+5)));
-    store1(buf+constr:(18+6), load1(buf+constr:(8+6)));
-    store1(buf+constr:(18+7), load1(buf+constr:(8+7)));
-    store1(buf+constr:(18+8), load1(buf+constr:(8+8)));
-    store1(buf+constr:(18+9), load1(buf+constr:(8+9)));
+    store1(ethbuf+constr:(14+18  ), load1(ethbuf+constr:(14+8  )));
+    store1(ethbuf+constr:(14+18+1), load1(ethbuf+constr:(14+8+1)));
+    store1(ethbuf+constr:(14+18+2), load1(ethbuf+constr:(14+8+2)));
+    store1(ethbuf+constr:(14+18+3), load1(ethbuf+constr:(14+8+3)));
+    store1(ethbuf+constr:(14+18+4), load1(ethbuf+constr:(14+8+4)));
+    store1(ethbuf+constr:(14+18+5), load1(ethbuf+constr:(14+8+5)));
+    store1(ethbuf+constr:(14+18+6), load1(ethbuf+constr:(14+8+6)));
+    store1(ethbuf+constr:(14+18+7), load1(ethbuf+constr:(14+8+7)));
+    store1(ethbuf+constr:(14+18+8), load1(ethbuf+constr:(14+8+8)));
+    store1(ethbuf+constr:(14+18+9), load1(ethbuf+constr:(14+8+9)));
 
     (* eth_dst = src *)
-    store1(ethbuf           , load1(buf+constr:(8  )));
-    store1(ethbuf+constr:(1), load1(buf+constr:(8+1)));
-    store1(ethbuf+constr:(2), load1(buf+constr:(8+2)));
-    store1(ethbuf+constr:(3), load1(buf+constr:(8+3)));
-    store1(ethbuf+constr:(4), load1(buf+constr:(8+4)));
-    store1(ethbuf+constr:(5), load1(buf+constr:(8+5)));
+    store1(ethbuf           , load1(ethbuf+constr:(14+8  )));
+    store1(ethbuf+constr:(1), load1(ethbuf+constr:(14+8+1)));
+    store1(ethbuf+constr:(2), load1(ethbuf+constr:(14+8+2)));
+    store1(ethbuf+constr:(3), load1(ethbuf+constr:(14+8+3)));
+    store1(ethbuf+constr:(4), load1(ethbuf+constr:(14+8+4)));
+    store1(ethbuf+constr:(5), load1(ethbuf+constr:(14+8+5)));
 
     (* src := me *)
-    store1(buf+constr:(8  ), constr:(Ox"f0"));
-    store1(buf+constr:(8+1), constr:(Ox"f1"));
-    store1(buf+constr:(8+2), constr:(Ox"f2"));
-    store1(buf+constr:(8+3), constr:(Ox"f3"));
-    store1(buf+constr:(8+4), constr:(Ox"f4"));
-    store1(buf+constr:(8+5), constr:(Ox"f5"));
-    store1(buf+constr:(8+6), constr:( 10));
-    store1(buf+constr:(8+7), constr:(155));
-    store1(buf+constr:(8+8), constr:(  5));
-    store1(buf+constr:(8+9), constr:(  1));
+    store1(ethbuf+constr:(14+8  ), constr:(Ox"f0"));
+    store1(ethbuf+constr:(14+8+1), constr:(Ox"f1"));
+    store1(ethbuf+constr:(14+8+2), constr:(Ox"f2"));
+    store1(ethbuf+constr:(14+8+3), constr:(Ox"f3"));
+    store1(ethbuf+constr:(14+8+4), constr:(Ox"f4"));
+    store1(ethbuf+constr:(14+8+5), constr:(Ox"f5"));
+    store1(ethbuf+constr:(14+8+6), constr:( 10));
+    store1(ethbuf+constr:(14+8+7), constr:(155));
+    store1(ethbuf+constr:(14+8+8), constr:(  5));
+    store1(ethbuf+constr:(14+8+9), constr:(  1));
 
     (* eth_src = me *)
     store1(ethbuf+constr:(6+0), constr:(Ox"f0"));
