bedrock2/src/Examples/ARPResponderProofs.v
@@ -1,0 +1,132 @@
+From Coq Require Import Strings.String Lists.List ZArith.BinInt.
+From bedrock2 Require Import BasicC64Semantics ProgramLogic.
+
+Require Import bedrock2.Examples.ARPResponder.
+
+Import ListNotations.
+Local Open Scope string_scope. Local Open Scope list_scope. Local Open Scope Z_scope.
+Require Import bedrock2.NotationsInConstr.
+From coqutil.Word Require Import Interface.
+
+From bedrock2 Require Import Array Scalars Separation.
+From coqutil.Tactics Require Import letexists rdelta.
+Local Notation bytes := (array scalar8 (word.of_Z 1)).
+
+Lemma word__if_zero (t:bool) (H : word.unsigned (if t then word.of_Z 1 else word.of_Z 0) = 0) : t = false. Admitted.
+Lemma word__if_nonzero (t:bool) (H : word.unsigned (if t then word.of_Z 1 else word.of_Z 0) <> 0) : t = true. Admitted.
+
+Set Printing Width 90.
+Ltac seplog_use_array_load1 H i :=
+  let iNat := eval cbv in (Z.to_nat i) in
+  unshelve SeparationLogic.seprewrite_in @array_index_nat_inbounds H;
+    [exact iNat|exact (word.of_Z 0)|Lia.lia|];
+  change ((word.unsigned (word.of_Z 1) * Z.of_nat iNat)%Z) with i in *.
+
+Local Instance spec_of_arp : spec_of "arp" := fun functions =>
+  forall t m packet ethbuf len R,
+    (sep (array scalar8 (word.of_Z 1) ethbuf packet) R) m ->
+    word.unsigned len = Z.of_nat (length packet) ->
+  WeakestPrecondition.call functions "arp" t m [ethbuf; len] (fun T M rets => True).
+Goal program_logic_goal_for_function! arp.
+  repeat straightline.
+  letexists; split; [solve[repeat straightline]|]; split; [|solve[repeat straightline]]; repeat straightline.
+  eapply word__if_nonzero in H1.
+  rewrite word.unsigned_ltu, word.unsigned_of_Z, Z.mod_small in H1 by admit.
+  eapply Z.ltb_lt in H1.
+  repeat (letexists || straightline).
+  split.
+  1: repeat (split || letexists || straightline).
+  Ltac tload := 
+  lazymatch goal with |- Memory.load Syntax.access_size.one ?m (word.add ?base (word.of_Z ?i)) = Some ?v =>
+  lazymatch goal with H: _ m |- _ =>
+    let iNat := eval cbv in (Z.to_nat i) in
+    SeparationLogic.seprewrite_in @array_index_nat_inbounds H;
+    [instantiate (1 := iNat); Lia.lia|instantiate (1 := word.of_Z 0) in H];
+    eapply load_one_of_sep;
+    simple refine (Lift1Prop.subrelation_iff1_impl1 _ _ _ _ _ H); clear H;
+    SeparationLogic.cancel;
+    simple refine (SeparationLogic.cancel_seps_at_indices 1 0 _ _ _ _); cbn [id];
+      eapply RelationClasses.reflexivity
+  end end.
+  all: try tload.
+  1: { straightline. }
+  split; [|solve[repeat straightline]]; repeat straightline.
+  
+  letexists; split.
+  1: repeat (split || letexists || straightline).
+  all: try tload.
+  1: { straightline. }
+  split; [|solve[repeat straightline]]; repeat straightline.
+
+  lazymatch goal with |- WeakestPrecondition.store Syntax.access_size.one ?m ?a ?v ?post =>
+  lazymatch goal with H: _ m |- _ =>
+    cbv [WeakestPrecondition.store];
+      eapply store_one_of_sep;
+    let a := rdelta a in
+    let i := lazymatch a with word.add ?base (word.of_Z ?i) => i end in
+    let iNat := eval cbv in (Z.to_nat i) in
+    SeparationLogic.seprewrite_in @array_index_nat_inbounds H;
+    [instantiate (1 := iNat); Lia.lia|instantiate (1 := word.of_Z 0) in H]
+  end end.
+  1: {
+    simple refine (Lift1Prop.subrelation_iff1_impl1 _ _ _ _ _ H); clear H;
+    SeparationLogic.cancel;
+    simple refine (SeparationLogic.cancel_seps_at_indices 1 0 _ _ _ _); cbn [id];
+      eapply RelationClasses.reflexivity. }
+
+  (* FIXME: make SeparationLogic.ecancel not reduce list functions *)
+  
+ (*  ============================ *)
+ (*  forall m0 : Interface.map.rep, *)
+ (*  sep (scalar8 a (word.of_Z (word.unsigned v2))) *)
+ (*    (fun m1 : Interface.map.rep => *)
+ (*     exists mp mq : Interface.map.rep, *)
+ (*       Interface.map.split m1 mp mq /\ *)
+ (*       bytes ethbuf (firstn 21 packet) mp /\ *)
+ (*       (fix seps (xs : list (Interface.map.rep -> Prop)) : Interface.map.rep -> Prop := *)
+ (*          match xs with *)
+ (*          | [] => emp True *)
+ (*          | [x] => x *)
+ (*          | x :: (_ :: _) as xs0 => sep x (seps xs0) *)
+ (*          end) *)
+ (*         ((fix app (l0 m2 : list (Interface.map.rep -> Prop)) {struct l0} : *)
+ (*             list (Interface.map.rep -> Prop) := *)
+ (*             match l0 with *)
+ (*             | [] => m2 *)
+ (*             | a0 :: l1 => a0 :: app l1 m2 *)
+ (*             end) *)
+ (*            ((fix firstn (n : nat) (l0 : list (Interface.map.rep -> Prop)) {struct n} : *)
+ (*                list (Interface.map.rep -> Prop) := *)
+ (*                match n with *)
+ (*                | 0%nat => [] *)
+ (*                | S n0 => match l0 with *)
+ (*                          | [] => [] *)
+ (*                          | a0 :: l1 => a0 :: firstn n0 l1 *)
+ (*                          end *)
+ (*                end) 0%nat *)
+ (*               [scalar8 *)
+ (*                  (word.add ethbuf *)
+ (*                     (word.of_Z (word.unsigned (word.of_Z 1) * Z.of_nat 21))) *)
+ (*                  (hd (word.of_Z 0) (skipn 21 packet)); *)
+ (*               bytes *)
+ (*                 (word.add *)
+ (*                    (word.add ethbuf *)
+ (*                       (word.of_Z (word.unsigned (word.of_Z 1) * Z.of_nat 21))) *)
+ (*                    (word.of_Z 1)) (tl (skipn 21 packet)); R]) *)
+ (*            (tl *)
+ (*               (skipn 1 *)
+ (*                  [bytes ethbuf (firstn 21 packet); *)
+ (*                  scalar8 *)
+ (*                    (word.add ethbuf *)
+ (*                       (word.of_Z (word.unsigned (word.of_Z 1) * Z.of_nat 21))) *)
+ (*                    (hd (word.of_Z 0) (skipn 21 packet)); *)
+ (*                  bytes *)
+ (*                    (word.add *)
+ (*                       (word.add ethbuf *)
+ (*                          (word.of_Z (word.unsigned (word.of_Z 1) * Z.of_nat 21))) *)
+ (*                       (word.of_Z 1)) (tl (skipn 21 packet)); R]))) mq) m0 -> *)
+ (*  WeakestPrecondition.cmd (WeakestPrecondition.call functions) c30 t m0 l *)
+ (*    (fun (_ : Semantics.trace) (_ l0 : Interface.map.rep) => *)
+ (*     WeakestPrecondition.list_map (WeakestPrecondition.get l0) [] *)
+ (*       (fun _ : list Semantics.word => True)) *)
+Abort.
